Some updated to Eucl

examples/Euclidean_Algorithm.thy
@@ -2,11 +2,46 @@ theory Euclidean_Algorithm
   imports "../ITree_Extraction"
 begin lit_vars
 
+datatype (discs_sels) ('inp, 'outp) MethodOp = Call_C 'inp | Return_C 'outp
+
+definition [lens_defs]: "Call = ctor_prism Call_C is_Call_C un_Call_C"
+definition [lens_defs]: "Return = ctor_prism Return_C (Not \<circ> is_Call_C) un_Return_C"
+
+lemma Call_wb_prism [simp, code_unfold]: "wb_prism Call" by (unfold_locales, auto simp add: lens_defs)
+lemma Return_wb_prism [simp, code_unfold]: "wb_prism Return" by (unfold_locales, auto simp add: lens_defs)
+
 alphabet gcd = 
   a :: integer
   b :: integer
 
-definition eucl_gcd :: "(_, gcd) htree" where
-"eucl_gcd = while a \<noteq> b do if a > b then a := a - b else b := b - a fi od"
+record_default gcd
+
+definition eucl :: "((integer \<times> integer, integer) MethodOp, gcd) htree" where
+"eucl = Call?(A, B) \<rightarrow> (a, b) := (A, B) \<Zcomp> while a \<noteq> b do if a > b then a := a - b else b := b - a fi od \<Zcomp> Return!(a) \<rightarrow> Skip"
+
+definition eucl_gcd where "eucl_gcd = proc [\<leadsto>] (eucl \<box> Stop)"
+
+definition inp' :: "('a \<Longrightarrow>\<^sub>\<triangle> 'e)\<Rightarrow> ('e, 'a) itree" where
+"inp' c = Vis (pfun_of_map (\<lambda> e. case match\<^bsub>c\<^esub> e of Some v \<Rightarrow> Some (Ret v) | None \<Rightarrow> None))"
+
+definition "input' c P = (\<lambda>s. inp' c \<bind> (\<lambda>x. P x s))"
+
+lemma inp_in_coset [code_unfold]: 
+  "wb_prism c \<Longrightarrow> inp_in c (List.coset []) = Vis (pfun_of_map (\<lambda> e. case match\<^bsub>c\<^esub> e of Some v \<Rightarrow> Some (Ret v) | None \<Rightarrow> None))"
+  by (auto simp add: inp_in_def pabs_def pfun_entries_def pdom_res_def pfun_of_map_inject restrict_map_def fun_eq_iff domIff wb_prism.range_build)
+
+lemma input_code_unfold [code_unfold]: 
+  "wb_prism c \<Longrightarrow> input c P = input' c P"
+  using inp_in_coset by (fastforce simp add: input_def input'_def inp_in_coset inp'_def)
+
+lemma map_pfun_of_map [code]: "map_pfun f (pfun_of_map g) = pfun_of_map (\<lambda> x. map_option f (g x))"
+  by (auto simp add: map_pfun_def pfun_of_map_inject fun_eq_iff)
+
+lemma "map_prod (pfun_of_map f) (pfun_of_map g) = undefined"
+
+
+text \<open> We need better code equations for @{const map_prod} for this to work\<close>
+
+export_code eucl_gcd in Haskell module_name Euclidean_Algorithm (string_classes)
 
 end
